\documentclass[a4paper]{article}
\usepackage{amsfonts}
\usepackage{amsmath}
\usepackage{amssymb}
\usepackage{graphicx}     

\begin{document}
  
\noindent \large Auteur: Muaz Moin\\
\noindent \large Studierichting: Informatica\\
\noindent \large Oefeningenreeks 1B nr. 44.2\\

\medskip

\normalsize

$z^4-5(1+2i)z^2+24-10i=0$\\

Stel: $x=z^2$\\

dan is $x^2-(5-10i)x+24-10i=0$\\

Hieruit volgt dat:

$D_1 = \left(x + yi\right)^2 = -171 + 140i$\\

$x^2 - y = -171 \Rightarrow x^2 - y^2 = -171$\\

$xy = 70 \Rightarrow x^2 \left( - y^2\right) = -4900$\\

$\lambda^2 + 171\lambda - 4900 = 0$\\

$D_2 = \left(171\right)^2 - 4 \cdot \left(-4900\right) = 48841$\\

$\rightarrow\lambda_1 = \dfrac{-171 + 221}{2} = 25 = \left(x^2\right)$\\

$\rightarrow\lambda_2 = \dfrac{-171 - 221}{2} = -196= \left(-y^2\right) $\\

$\Rightarrow \sqrt{D} \in \{ 5+14i, -5 - 14i\}$\\

$w_1 = \dfrac{5 + 10i + \left(5 + 14i \right)}{2} = 5 + 12i$\\

$w_2 = \dfrac{5 + 10i - \left(5 + 14i \right)}{2} = -2i $\\

Hierdoor weten we: $z^2 = -2i$ of $z^2 = 5 + 12i$\\

$z^2 = \left( x + yi\right)^2 = 5+12i$\\

    $\Rightarrow\left\{
	\begin{array}{l}
		x^2 - y^2 = 5\\
		xy = 6\\
	\end{array}
    \right .$\\

    $\Rightarrow\left\{
	\begin{array}{l}
		x^2 - y^2 = 5\\
		x^2 \left(-y^2\right) = -36\\
	\end{array}
    \right .$\\

$\lambda^2 - 5\lambda - 36 = 0$\\

$\Rightarrow\lambda_1 = 9 = x^2$\\

$\Rightarrow\lambda_2 = -4 = \left(-y\right)^2$\\

Hieruit volgt: $z = 3 + 2i$ of $z = -3 - 2i$ of $z^2 = -2i$\\

$z^2 = \left(x + yi \right) = -2i$\\

    $\Rightarrow\left\{
	\begin{array}{l}
		x^2 - y^2 = 0\\
		xy = -1\\
	\end{array}
    \right .$\\

    $\Rightarrow\left\{
	\begin{array}{l}
		x^2 - y^2 = 0\\
		x^2 \left(-y^2\right) = 7\\
	\end{array}
    \right .$\\

    
$\lambda - 0\lambda - 1 = 0$\\

$\Rightarrow\lambda_1 = 1 = x^2$\\

$\Rightarrow\lambda_2 = -1 = \left(-y\right)^2$\\

Hieruit lijden we het volgende af: \\
$\Rightarrow z = 3 + 2i$ of $z = -3 - 2i$ of $z = -1 + i$ of $z = 1 - i$\\

$\bold {Dus:}$

$z \in \{3 + 2i, -3 - 2i, -1 + i, 1 - i\}$
    



\begin{thebibliography}{999}
%\bibitem{a} Referentie
\end{thebibliography}
\end{document} 
